tests/List.bpl
@@ -27,32 +27,26 @@ var AT#intlst: List int;
 procedure ListTest#anon$0#0()
   modifies C, R, M, St;
 {
-  var x: List (int);
-  var i: int;
-  assume x[0] == 10;
-  assume (0 <= i) && (i < 3);
-  x[i] := 11;
-  assert {:msg "  3.13: Action might not preserve invariant"} x[0] == 10;
-}
-procedure Net#init#1()
-  modifies C, R, M, St;
-{
-  assume C[Net#a] == 0;
-  assume R[Net#a] == 0;
-  assume C[Net#b] == 0;
-  assume R[Net#b] == 0;
+  var X: List (int);
+  var IV#in#i: int;
+  var ActionVar#o: int;
+  assume (X[0] == 10) && (X[1] == 11) && (X[2] == 12);
+  assume (0 <= IV#in#i) && (IV#in#i < 3);
+  ActionVar#o := X[IV#in#i];
+  assert {:msg "  3.13: Action might not preserve invariant"} (X[0] == 10) && (X[1] == 11) && (X[2] == 12);
 }
 const unique Net#l: Actor;
 const unique Net#a: Chan (int);
 const unique Net#b: Chan (int);
-procedure Net#anon$1#entry#2()
+procedure Net#anon$1#entry#1()
   modifies C, R, M, St;
 {
+  var ActionVar#y: int;
   assume C#init[Net#a] == 1;
   assume C#init[Net#b] == 0;
   assume R[Net#a] == 0;
   assume R[Net#b] == 0;
-  assume M[Net#a][0] == 0;
+  assume (0 <= M[Net#a][0]) && (M[Net#a][0] < 3);
   assume C#init == C;
   assert {:msg "  Channel invariant might not hold on action entry (generated #0)"} 0 <= R[Net#a];
   assert {:msg "  Channel invariant might not hold on action entry (generated #1)"} 0 <= C[Net#a];
@@ -60,16 +54,20 @@ procedure Net#anon$1#entry#2()
   assert {:msg "  Channel invariant might not hold on action entry (generated #3)"} 0 <= R[Net#b];
   assert {:msg "  Channel invariant might not hold on action entry (generated #4)"} 0 <= C[Net#b];
   assert {:msg "  Channel invariant might not hold on action entry (generated #5)"} R[Net#b] == 0;
-  assert {:msg "  19.3: Channel invariant might not hold on action entry"} M[Net#a][0] == 0;
-  assert {:msg "  20.3: Channel invariant might not hold on action entry"} R[Net#a] == (R[Net#b] + C[Net#b]);
-  assert {:msg "  21.3: Channel invariant might not hold on action entry"} (forall i: int :: 
-    (0 <= i) && (i < (R[Net#b] + C[Net#b])) ==> (M[Net#b][i] == 10)
+  assert {:msg "  22.3: Channel invariant might not hold on action entry"} (0 <= M[Net#a][0]) && (M[Net#a][0] < 3);
+  assert {:msg "  23.3: Channel invariant might not hold on action entry"} R[Net#a] == (R[Net#b] + C[Net#b]);
+  assert {:msg "  24.3: Channel invariant might not hold on action entry"} (forall i: int :: 
+    (0 <= i) && (i < (R[Net#b] + C[Net#b])) ==> (10 <= M[Net#b][i]) && (M[Net#b][i] <= 12)
+  );
+  assert {:msg "  25.3: Channel invariant might not hold on action entry"} (forall i: int :: 
+    (0 <= i) && (i < (R[Net#b] + C[Net#b])) ==> ((M[Net#a][i] == 0) ==> (M[Net#b][i] == 10))
   );
 }
-procedure Net#anon$1#ListTest#anon$0#3()
+procedure Net#anon$1#ListTest#anon$0#2()
   modifies C, R, M, St;
 {
-  var ActorVar#x: List (int);
+  var ActorVar#X: List (int);
+  var ActionVar#o: int;
   var St#next: State;
   var in#i: int;
   assume C#init[Net#a] == 1;
@@ -80,19 +78,22 @@ procedure Net#anon$1#ListTest#anon$0#3()
   assume 0 <= R[Net#b];
   assume 0 <= C[Net#b];
   assume R[Net#b] == 0;
-  assume M[Net#a][0] == 0;
+  assume (0 <= M[Net#a][0]) && (M[Net#a][0] < 3);
   assume R[Net#a] == (R[Net#b] + C[Net#b]);
   assume (forall i: int :: 
-    (0 <= i) && (i < (R[Net#b] + C[Net#b])) ==> (M[Net#b][i] == 10)
+    (0 <= i) && (i < (R[Net#b] + C[Net#b])) ==> (10 <= M[Net#b][i]) && (M[Net#b][i] <= 12)
+  );
+  assume (forall i: int :: 
+    (0 <= i) && (i < (R[Net#b] + C[Net#b])) ==> ((M[Net#a][i] == 0) ==> (M[Net#b][i] == 10))
   );
   assume (0 <= M[Net#a][R[Net#a] - 0]) && (M[Net#a][R[Net#a] - 0] < 3);
   assume true;
   assume (1 <= C[Net#a]) && (0 <= M[Net#a][R[Net#a] - 0]) && (M[Net#a][R[Net#a] - 0] < 3);
-  assume ActorVar#x[0] == 10;
+  assume (ActorVar#X[0] == 10) && (ActorVar#X[1] == 11) && (ActorVar#X[2] == 12);
   in#i := M[Net#a][R[Net#a]];
   R[Net#a] := R[Net#a] + 1;
   C[Net#a] := C[Net#a] - 1;
-  M[Net#b][R[Net#b] + C[Net#b]] := ActorVar#x[in#i];
+  M[Net#b][R[Net#b] + C[Net#b]] := ActorVar#X[in#i];
   C[Net#b] := C[Net#b] + 1;
   assert {:msg "  Sub-actor action at 7.3 might not preserve the channel invariant (generated #6)"} 0 <= R[Net#a];
   assert {:msg "  Sub-actor action at 7.3 might not preserve the channel invariant (generated #7)"} 0 <= C[Net#a];
@@ -100,15 +101,19 @@ procedure Net#anon$1#ListTest#anon$0#3()
   assert {:msg "  Sub-actor action at 7.3 might not preserve the channel invariant (generated #9)"} 0 <= R[Net#b];
   assert {:msg "  Sub-actor action at 7.3 might not preserve the channel invariant (generated #10)"} 0 <= C[Net#b];
   assert {:msg "  Sub-actor action at 7.3 might not preserve the channel invariant (generated #11)"} R[Net#b] == 0;
-  assert {:msg "  19.3: Sub-actor action at 7.3 might not preserve the channel invariant"} M[Net#a][0] == 0;
-  assert {:msg "  20.3: Sub-actor action at 7.3 might not preserve the channel invariant"} R[Net#a] == (R[Net#b] + C[Net#b]);
-  assert {:msg "  21.3: Sub-actor action at 7.3 might not preserve the channel invariant"} (forall i: int :: 
-    (0 <= i) && (i < (R[Net#b] + C[Net#b])) ==> (M[Net#b][i] == 10)
+  assert {:msg "  22.3: Sub-actor action at 7.3 might not preserve the channel invariant"} (0 <= M[Net#a][0]) && (M[Net#a][0] < 3);
+  assert {:msg "  23.3: Sub-actor action at 7.3 might not preserve the channel invariant"} R[Net#a] == (R[Net#b] + C[Net#b]);
+  assert {:msg "  24.3: Sub-actor action at 7.3 might not preserve the channel invariant"} (forall i: int :: 
+    (0 <= i) && (i < (R[Net#b] + C[Net#b])) ==> (10 <= M[Net#b][i]) && (M[Net#b][i] <= 12)
+  );
+  assert {:msg "  25.3: Sub-actor action at 7.3 might not preserve the channel invariant"} (forall i: int :: 
+    (0 <= i) && (i < (R[Net#b] + C[Net#b])) ==> ((M[Net#a][i] == 0) ==> (M[Net#b][i] == 10))
   );
 }
-procedure Net#anon$1#exit#4()
+procedure Net#anon$1#exit#3()
   modifies C, R, M, St;
 {
+  var ActionVar#y: int;
   assume C#init[Net#a] == 1;
   assume C#init[Net#b] == 0;
   assume 0 <= R[Net#a];
@@ -117,15 +122,19 @@ procedure Net#anon$1#exit#4()
   assume 0 <= R[Net#b];
   assume 0 <= C[Net#b];
   assume R[Net#b] == 0;
-  assume M[Net#a][0] == 0;
+  assume (0 <= M[Net#a][0]) && (M[Net#a][0] < 3);
   assume R[Net#a] == (R[Net#b] + C[Net#b]);
   assume (forall i: int :: 
-    (0 <= i) && (i < (R[Net#b] + C[Net#b])) ==> (M[Net#b][i] == 10)
+    (0 <= i) && (i < (R[Net#b] + C[Net#b])) ==> (10 <= M[Net#b][i]) && (M[Net#b][i] <= 12)
+  );
+  assume (forall i: int :: 
+    (0 <= i) && (i < (R[Net#b] + C[Net#b])) ==> ((M[Net#a][i] == 0) ==> (M[Net#b][i] == 10))
   );
   assume !((1 <= C[Net#a]) && (0 <= M[Net#a][R[Net#a] - 0]) && (M[Net#a][R[Net#a] - 0] < 3));
-  assert {:msg "  15.3: The network might leave unread tokens on channel a"} C[Net#a] == 0;
-  assert {:msg "  15.3: The network might not produce the specified number of tokens on output out"} C[Net#b] == 1;
-  assert {:msg "  15.26: Network output might not conform to specified action output"} M[Net#b][0] == 10;
+  assert {:msg "  16.3: The network might leave unread tokens on channel a"} C[Net#a] == 0;
+  assert {:msg "  16.3: The network might not produce the specified number of tokens on output out"} C[Net#b] == 1;
+  ActionVar#y := M[Net#b][0];
+  assert {:msg "  19.14: Postcondition might not hold"} (M[Net#a][0] == 0) ==> (ActionVar#y == 10);
   R[Net#b] := R[Net#b] + C[Net#b];
   C[Net#b] := 0;
 }
