tests/Nested.bpl
@@ -13,7 +13,12 @@ var R: CType;
 var C#init: CType;
 var St: [Actor]State;
 
+
 const unique this#: Actor;
+
+type List a = [int]a;
+var AT#intlst: List int;
+
 
 // ---------------------------------------------------------------
 // -- End of prelude ---------------------------------------------
@@ -25,17 +30,18 @@ const unique Top#y: Chan (int);
 procedure Top#anon$0#entry#0()
   modifies C, R, M, St;
 {
+  var Top#out#0: int;
   assume C#init[Top#x] == 1;
   assume C#init[Top#y] == 0;
   assume R[Top#x] == 0;
   assume R[Top#y] == 0;
   assume C#init == C;
-  assert {:msg "  Channel invariant might not hold on action entry (generated #0 )"} 0 <= R[Top#x];
-  assert {:msg "  Channel invariant might not hold on action entry (generated #1 )"} 0 <= C[Top#x];
-  assert {:msg "  Channel invariant might not hold on action entry (generated #2 )"} (R[Top#x] + C[Top#x]) == C#init[Top#x];
-  assert {:msg "  Channel invariant might not hold on action entry (generated #3 )"} 0 <= R[Top#y];
-  assert {:msg "  Channel invariant might not hold on action entry (generated #4 )"} 0 <= C[Top#y];
-  assert {:msg "  Channel invariant might not hold on action entry (generated #5 )"} R[Top#y] == 0;
+  assert {:msg "  Channel invariant might not hold on action entry (generated #0)"} 0 <= R[Top#x];
+  assert {:msg "  Channel invariant might not hold on action entry (generated #1)"} 0 <= C[Top#x];
+  assert {:msg "  Channel invariant might not hold on action entry (generated #2)"} (R[Top#x] + C[Top#x]) == C#init[Top#x];
+  assert {:msg "  Channel invariant might not hold on action entry (generated #3)"} 0 <= R[Top#y];
+  assert {:msg "  Channel invariant might not hold on action entry (generated #4)"} 0 <= C[Top#y];
+  assert {:msg "  Channel invariant might not hold on action entry (generated #5)"} R[Top#y] == 0;
   assert {:msg "  4.3: Channel invariant might not hold on action entry"} (R[Top#y] + C[Top#y]) == R[Top#x];
   assert {:msg "  5.3: Channel invariant might not hold on action entry"} (forall i: int :: 
     (0 <= i) && (i < (R[Top#y] + C[Top#y])) ==> (M[Top#x][i] == M[Top#y][i])
@@ -79,6 +85,7 @@ procedure Top#anon$0#Nested#anon$1#1()
 procedure Top#anon$0#exit#2()
   modifies C, R, M, St;
 {
+  var Top#out#0: int;
   assume C#init[Top#x] == 1;
   assume C#init[Top#y] == 0;
   assume 0 <= R[Top#x];
@@ -94,7 +101,8 @@ procedure Top#anon$0#exit#2()
   assume !(1 <= C[Top#x]);
   assert {:msg "  2.3: The network might leave unread tokens on channel x"} C[Top#x] == 0;
   assert {:msg "  2.3: The network might not produce the specified number of tokens on output out"} C[Top#y] == 1;
-  assert {:msg "  2.26: Network output might not conform to specified action output"} M[Top#y][0] == M[Top#x][0];
+  Top#out#0 := M[Top#y][0];
+  assert {:msg "  2.26: Network output might not conform to the specified action output"} Top#out#0 == M[Top#x][0];
   R[Top#y] := R[Top#y] + C[Top#y];
   C[Top#y] := 0;
 }
@@ -104,17 +112,18 @@ const unique Nested#y: Chan (int);
 procedure Nested#anon$1#entry#3()
   modifies C, R, M, St;
 {
+  var Nested#y#0: int;
   assume C#init[Nested#x] == 1;
   assume C#init[Nested#y] == 0;
   assume R[Nested#x] == 0;
   assume R[Nested#y] == 0;
   assume C#init == C;
-  assert {:msg "  Channel invariant might not hold on action entry (generated #12 )"} 0 <= R[Nested#x];
-  assert {:msg "  Channel invariant might not hold on action entry (generated #13 )"} 0 <= C[Nested#x];
-  assert {:msg "  Channel invariant might not hold on action entry (generated #14 )"} (R[Nested#x] + C[Nested#x]) == C#init[Nested#x];
-  assert {:msg "  Channel invariant might not hold on action entry (generated #15 )"} 0 <= R[Nested#y];
-  assert {:msg "  Channel invariant might not hold on action entry (generated #16 )"} 0 <= C[Nested#y];
-  assert {:msg "  Channel invariant might not hold on action entry (generated #17 )"} R[Nested#y] == 0;
+  assert {:msg "  Channel invariant might not hold on action entry (generated #12)"} 0 <= R[Nested#x];
+  assert {:msg "  Channel invariant might not hold on action entry (generated #13)"} 0 <= C[Nested#x];
+  assert {:msg "  Channel invariant might not hold on action entry (generated #14)"} (R[Nested#x] + C[Nested#x]) == C#init[Nested#x];
+  assert {:msg "  Channel invariant might not hold on action entry (generated #15)"} 0 <= R[Nested#y];
+  assert {:msg "  Channel invariant might not hold on action entry (generated #16)"} 0 <= C[Nested#y];
+  assert {:msg "  Channel invariant might not hold on action entry (generated #17)"} R[Nested#y] == 0;
   assert {:msg "  19.3: Channel invariant might not hold on action entry"} (R[Nested#y] + C[Nested#y]) == R[Nested#x];
   assert {:msg "  20.3: Channel invariant might not hold on action entry"} (forall i: int :: 
     (0 <= i) && (i < (R[Nested#y] + C[Nested#y])) ==> (M[Nested#x][i] == M[Nested#y][i])
@@ -158,6 +167,7 @@ procedure Nested#anon$1#Repeater#anon$2#4()
 procedure Nested#anon$1#exit#5()
   modifies C, R, M, St;
 {
+  var Nested#y#0: int;
   assume C#init[Nested#x] == 1;
   assume C#init[Nested#y] == 0;
   assume 0 <= R[Nested#x];
@@ -173,13 +183,14 @@ procedure Nested#anon$1#exit#5()
   assume !(1 <= C[Nested#x]);
   assert {:msg "  17.3: The network might leave unread tokens on channel x"} C[Nested#x] == 0;
   assert {:msg "  17.3: The network might not produce the specified number of tokens on output y"} C[Nested#y] == 1;
-  assert {:msg "  17.23: Network output might not conform to specified action output"} M[Nested#y][0] == M[Nested#x][0];
+  Nested#y#0 := M[Nested#y][0];
+  assert {:msg "  17.23: Network output might not conform to the specified action output"} Nested#y#0 == M[Nested#x][0];
   R[Nested#y] := R[Nested#y] + C[Nested#y];
   C[Nested#y] := 0;
 }
 procedure Repeater#anon$2#6()
   modifies C, R, M, St;
 {
-  var i: int;
+  var IV#in#i: int;
   assume true;
 }
